gzk

generic/GenericZeroKnowledge.ec
@@ -26,7 +26,7 @@ module type ZKDistinguisher = {
 }.
 
 module type Simulator(V: RewMaliciousVerifier) = {
-  proc * simulate(statement: statement, n : int) : adv_summary
+  proc * simulate(statement: statement) : adv_summary
 }.
 
 module type Simulator1(V: RewMaliciousVerifier) = {
@@ -49,9 +49,9 @@ module ZKReal(P: HonestProver, V: MaliciousVerifier, D: ZKDistinguisher) = {
 
 
 module ZKIdeal(S: Simulator, V: RewMaliciousVerifier, D: ZKDistinguisher) = {
-  proc run(statement: statement, witness: witness, n : int) = {
+  proc run(statement: statement, witness: witness) = {
     var summary, guess;
-    summary <@ S(V).simulate(statement, n);
+    summary <@ S(V).simulate(statement);
     guess <@ D.guess(statement, witness, summary);
     return guess;
   }
@@ -59,18 +59,221 @@ module ZKIdeal(S: Simulator, V: RewMaliciousVerifier, D: ZKDistinguisher) = {
 
 
 
+abstract theory OneShotSimulator.
 
-abstract theory ZeroKnowledgeTheory.
+op zk_error : statement -> int -> real.
+op n : int.
+axiom n_pos : 0 <= n.
+
+require OneToManyZK.
+clone import OneToManyZK as OMZK with type prob <- statement,
+                                      type wit <- witness,
+                                      type sbits <- adv_summary,
+                                      type event <- bool,
+                                      op E <- fst,
+                                      op fevent <- false
+
+rename "Simulator1" as "Simulator1NP".
+
+
+module ZKD(P : HonestProver, V : MaliciousVerifier, D : ZKDistinguisher) = {
+  proc main(Ny : statement, w : witness) = {
+    var c,b,r,result,rb;
+    c <@ P.commitment(Ny,w);
+    b <@ V.challenge(Ny,c);
+    r <@ P.response(b);
+    result <@ V.summitup(Ny,r);
+    rb <@ D.guess(Ny,w,result);
+    return rb;
+  }
+}.
+
+
+module  Simulator(S : Simulator1)(V : RewMaliciousVerifier)  = {
+  module M = MW.IFB.IM.W(S(V))
+  proc simulate(statement : statement) :
+    adv_summary = {
+       var r;
+       r <@ M.whp(fst,statement,1,n,(false,witness));
+       return r.`2;
+  }
+}.
+
+   theory ComputationalZK.
+
+   section.
+
+   declare module HonestProver <: HonestProver.
+   declare module Sim1 <: Simulator1 {-MW.IFB.IM.W, -MW.IFB.DW}.
+   declare module V <: RewMaliciousVerifier {-Sim1, -MW.IFB.IM.W, -HonestProver, -MW.IFB.DW}.
+   declare module D <: ZKDistinguisher{ -MW.IFB.DW, -MW.IFB.IM.W} .
+
+   declare axiom sim1_run_ll : forall (V0 <: RewMaliciousVerifier),
+        islossless V0.challenge => islossless V0.summitup => islossless Sim1(V0).run.
+   declare axiom V_summitup_ll  : islossless V.summitup.
+   declare axiom V_challenge_ll : islossless V.challenge.
+   declare axiom D_guess_ll     : islossless D.guess.
+
+
+   declare axiom V_rew :  (exists (f : glob V -> sbits),
+        injective f /\
+        (forall &m, Pr[ V.getState() @ &m : (glob V) = ((glob V){m})
+                                         /\ res = f ((glob V){m} ) ] = 1%r) /\
+        (forall &m b (x: glob V), b = f x =>
+          Pr[V.setState(b) @ &m : glob V = x] = 1%r) /\
+        islossless V.setState).
+
+
+   declare axiom sim1_rew_ph : forall (x : (glob Sim1(V))),
+                 phoare[ Sim1(V).run : (glob Sim1(V)) = x ==> ! fst res => (glob Sim1(V)) = x] = 1%r.
+
+
+   declare axiom D_guess_prop : equiv[ D.guess ~ D.guess : ={glob V, arg} ==> ={res} ].
+
+    lemma computational_statisticalVpoly_zk stat wit p0 negl &m:
+       zk_relation stat wit =>
+       `|Pr[W0(Sim1(V), D).run(stat, wit) @ &m : fst res.`2 /\ res.`1] /
+            Pr[Sim1(V).run(stat) @ &m : fst res]
+        - Pr[ ZKD(HonestProver,V,D).main(stat,wit) @ &m : res ]| <= negl =>
+
+       p0 <= Pr[Sim1(V).run(stat) @ &m : res.`1] =>
+
+       let real_prob = Pr[ZKReal(HonestProver, V, D).run(stat, wit) @ &m : res] in
+       let ideal_prob = Pr[ZKIdeal(Simulator(Sim1), V, D).run(stat, wit) @ &m : res] in
+         `|real_prob - ideal_prob| <= negl + 2%r * (1%r - p0)^n.
+   proof. progress.
+   have ->:
+    `|Pr[ZKReal(HonestProver, V, D).run(stat, wit) @ &m : res] -
+     Pr[ZKIdeal(Simulator(Sim1), V, D).run(stat, wit) @ &m : res]|
+     = `|Pr[ZKIdeal(Simulator(Sim1), V, D).run(stat, wit) @ &m : res]
+         - Pr[ZKReal(HonestProver, V, D).run(stat, wit) @ &m : res]|. smt.
+   have ->: Pr[ZKIdeal(Simulator(Sim1), V, D).run(stat, wit) @ &m : res]
+    = Pr[Iter(Sim1(V), D).run(false,stat,wit,n,fst) @ &m : res.`1].
+   byequiv (_:  E{2} = fst  /\ n{1} = ea{2} /\ fevent{2} = false  /\
+     statement{1} = Ny{2} /\ witness{1} = w{2} /\
+       ={glob Sim1, glob HonestProver,  glob V, glob MW.IFB.IM.W} ==> _)  ;auto.  proc.
+   inline Iter(Sim1(V), D).WI.run. wp.  sp. simplify.
+    call D_guess_prop.
+   simplify. inline Simulator(Sim1,V).simulate. wp. sp.
+   call (_: ={glob Sim1, glob V, glob MW.IFB.IM.W}).  sim. skip. progress.
+   progress.
+   have ->: Pr[ZKReal(HonestProver, V, D).run(stat, wit) @ &m : res]
+     = Pr[ ZKD(HonestProver,V,D).main(stat,wit) @ &m : res ].
+    byequiv (_:   arg{2} = (stat, wit) /\ ={glob V, glob HonestProver}
+  /\
+  (glob V){2} = (glob V){m} /\
+  (glob HonestProver){2} = (glob HonestProver){m} /\
+  arg{1} = (stat, wit) /\
+  (glob V){1} = (glob V){m} /\
+  (glob HonestProver){1} = (glob HonestProver){m} ==> _).
+  proc. seq  4 4 : (={glob V} /\ (statement{1}, witness{1}, summary{1}) =
+  (Ny{2}, w{2}, result{2})). sim. call D_guess_prop. skip. auto. auto. auto.
+   apply (one_to_many_zk  (Sim1(V)) D _  _ _ _ _ &m  stat wit p0 negl n
+      Pr[ZKD(HonestProver, V, D).main(stat, wit) @ &m : res]  _ _ _).
+   conseq D_guess_prop. auto.
+   apply (sim1_run_ll V). apply V_challenge_ll. apply V_summitup_ll.
+   apply sim1_rew_ph. apply D_guess_ll.
+   auto. auto. apply n_pos. smt. auto.
+   qed.
+   end section.
+  end ComputationalZK.
+
+   
+  theory StatisticalZK.
+
+   op negl : real.
+
+   section.
+   declare module HonestProver <: HonestProver.
+   declare module Sim1 <: Simulator1 {-MW.IFB.IM.W, -MW.IFB.DW}.
+   declare module V <: RewMaliciousVerifier {-Sim1, -MW.IFB.IM.W, -HonestProver, -MW.IFB.DW}.
+   declare module D <: ZKDistinguisher{-MW.IFB.IM.W,  -MW.IFB.DW}.
+
+   declare axiom sim1_run_ll : forall (V0 <: RewMaliciousVerifier), islossless V0.challenge
+                                 => islossless V0.summitup => islossless Sim1(V0).run.
+   declare axiom V_summitup_ll  : islossless V.summitup.
+   declare axiom V_challenge_ll : islossless V.challenge.
+   declare axiom D_guess_ll     : islossless D.guess.
+
+   declare axiom V_rew :  (exists (f : glob V -> sbits),
+        injective f /\
+        (forall &m, Pr[ V.getState() @ &m : (glob V) = ((glob V){m})
+                                         /\ res = f ((glob V){m} ) ] = 1%r) /\
+        (forall &m b (x: glob V), b = f x =>
+          Pr[V.setState(b) @ &m : glob V = x] = 1%r) /\
+        islossless V.setState).
+
+
+   declare axiom sim1_rew_ph :
+        forall (x : (glob Sim1(V))),
+                 phoare[ Sim1(V).run : (glob Sim1(V)) = x ==> !fst res => (glob Sim1(V)) = x] = 1%r.
+
+
+   declare axiom qqq &m (p : statement) (w : witness)
+     (D <: ZKDistinguisher)
+        (V <: RewMaliciousVerifier{-D, -HonestProver}):
+      islossless D.guess =>
+      islossless V.summitup =>
+      islossless V.challenge =>
+     (exists (f : glob V -> sbits),
+        injective f /\
+        (forall &m, Pr[ V.getState() @ &m : (glob V) = ((glob V){m})
+                                         /\ res = f ((glob V){m} ) ] = 1%r) /\
+        (forall &m b (x: glob V), b = f x =>
+          Pr[V.setState(b) @ &m : glob V = x] = 1%r) /\
+        islossless V.setState) =>
+      zk_relation p w =>
+       `|Pr[W0(Sim1(V), D).run(p, w) @ &m : fst res.`2 /\ res.`1] /
+            Pr[Sim1(V).run(p) @ &m : fst res]
+                 - Pr[ ZKD(HonestProver,V,D).main(p,w) @ &m : res ]| <= negl.
+
+
+   declare axiom D_guess_prop : equiv[ D.guess ~ D.guess : ={glob V, arg} ==> ={res} ].
+
+    lemma statistical_zk stat wit p0 &m:
+       zk_relation stat wit => 
+       p0 <= Pr[Sim1(V).run(stat) @ &m : res.`1] =>
+       let real_prob = Pr[ZKReal(HonestProver, V, D).run(stat, wit) @ &m : res] in
+       let ideal_prob = Pr[ZKIdeal(Simulator(Sim1), V, D).run(stat, wit) @ &m : res] in
+         `|real_prob - ideal_prob| <= negl + 2%r * (1%r - p0)^n.
+   proof. progress.
+   have ->:
+    `|Pr[ZKReal(HonestProver, V, D).run(stat, wit) @ &m : res] -
+     Pr[ZKIdeal(Simulator(Sim1), V, D).run(stat, wit) @ &m : res]|
+     = `|Pr[ZKIdeal(Simulator(Sim1), V, D).run(stat, wit) @ &m : res]
+         - Pr[ZKReal(HonestProver, V, D).run(stat, wit) @ &m : res]|. smt.
+   have ->: Pr[ZKIdeal(Simulator(Sim1), V, D).run(stat, wit) @ &m : res]
+    = Pr[Iter(Sim1(V), D).run(false,stat,wit,n,fst) @ &m : res.`1].
+   byequiv (_:  E{2} = fst /\ n{1} = ea{2} /\ fevent{2} = false  /\
+     statement{1} = Ny{2} /\ witness{1} = w{2} /\
+       ={glob Sim1, glob HonestProver,  glob V, glob MW.IFB.IM.W} ==> _)  ;auto. proc.
+   inline Iter(Sim1(V), D).WI.run. wp.  sp. simplify.
+   call D_guess_prop.  simplify. inline Simulator(Sim1,V).simulate. wp. sp.
+   call (_: ={glob Sim1, glob V, glob MW.IFB.IM.W}).  sim. skip. progress.
+   have ->: Pr[ZKReal(HonestProver, V, D).run(stat, wit) @ &m : res]
+     = Pr[ ZKD(HonestProver,V,D).main(stat,wit) @ &m : res ].
+  byequiv(_: arg{2} = (stat,  wit) /\   arg{1} = (stat, wit) /\  ={glob V, glob HonestProver} ==> _).
+  proc. call D_guess_prop. sim. auto. auto.
+   apply (one_to_many_zk (Sim1(V)) D _ _ _ _ _ &m stat wit p0 negl n
+   Pr[ZKD(HonestProver, V, D).main(stat, wit) @
+  &m : res]  _ _ _
+  ) . conseq D_guess_prop. auto.
+  apply (sim1_run_ll V).  apply V_challenge_ll. apply V_summitup_ll. apply sim1_rew_ph. apply D_guess_ll. auto.
+   apply (qqq &m stat wit  D V);auto.  apply D_guess_ll. apply V_summitup_ll. apply V_challenge_ll. apply V_rew. apply n_pos. smt.  auto.
+   qed.
+  end section.
+  end StatisticalZK.
+end OneShotSimulator.
 
 
 
+abstract theory SequentialCompositionZK.
 
-op s:statement.
-op w:witness.
+op s : statement.
+op w : witness.
 op n : int.
 
 axiom zkrel_prop : zk_relation s w.
-
 
 module ZKRealAmp(P: HonestProver, V: MaliciousVerifier, D: ZKDistinguisher) = {
   proc run(statement: statement, witness: witness) = {
@@ -91,12 +294,12 @@ module ZKRealAmp(P: HonestProver, V: MaliciousVerifier, D: ZKDistinguisher) = {
 
 
 module SimAmp(S: Simulator, V : RewMaliciousVerifier) = { 
-  proc simulate(statement:statement,N : int) = { 
+  proc simulate(statement:statement) = { 
    var summary, i; 
    i <- 0;
    summary <- witness;
    while(i < n) { 
-     summary <@ S(V).simulate(statement, N); 
+     summary <@ S(V).simulate(statement); 
      i <- i + 1;
    } 
    return summary; 
@@ -141,7 +344,7 @@ module Obb(P : HonestProver, V : RewMaliciousVerifier, Sim : Simulator) = {
   }
   proc orclL() : adv_summary = {
     var summary;
-    summary <@ Sim(V).simulate(s, n);
+    summary <@ Sim(V).simulate(s);
     return summary;
   }
 }.
@@ -269,10 +472,10 @@ module Z3 = {
      summary <@ V.summitup(s, response);
      HybOrcl.l <- HybOrcl.l + 1;
    }
-   summary <@ Sim(V).simulate(s, n);
+   summary <@ Sim(V).simulate(s);
    HybOrcl.l <- HybOrcl.l + 1;
    while (HybOrcl.l < n) {
-    summary <@ Sim(V).simulate(s, n);
+    summary <@ Sim(V).simulate(s);
     HybOrcl.l <- HybOrcl.l + 1;
    }
    guess <@ D.guess(s, w, summary);
@@ -298,7 +501,7 @@ module Y3 = {
      summary <@ V.summitup(s, response);
    HybOrcl.l <- HybOrcl.l + 1;
    while (HybOrcl.l < n) {
-    summary <@ Sim(V).simulate(s, n);
+    summary <@ Sim(V).simulate(s);
     HybOrcl.l <- HybOrcl.l + 1;
    }
    guess <@ D.guess(s, w, summary);
@@ -516,10 +719,10 @@ module Amem : IR1R2 = {
   }
   proc run1() = {
    var  summary, guess;
-   summary <@ Sim(V).simulate(s, n);
+   summary <@ Sim(V).simulate(s);
    HybOrcl.l <- HybOrcl.l + 1;
    while (HybOrcl.l < n) {
-    summary <@ Sim(V).simulate(s, n);
+    summary <@ Sim(V).simulate(s);
     HybOrcl.l <- HybOrcl.l + 1;
    }
    guess <@ D.guess(s, w, summary);
@@ -533,7 +736,7 @@ module Amem : IR1R2 = {
    summary <@ V.summitup(s, response);
    HybOrcl.l <- HybOrcl.l + 1;
    while (HybOrcl.l < n) {
-    summary <@ Sim(V).simulate(s, n);
+    summary <@ Sim(V).simulate(s);
     HybOrcl.l <- HybOrcl.l + 1;
    }
    guess <@ D.guess(s, w, summary);
@@ -546,7 +749,7 @@ module Dstar : ZKDistinguisher = {
    var guess;
    HybOrcl.l <- HybOrcl.l + 1;
    while (HybOrcl.l < n) {
-    summary <@ Sim(V).simulate(s, n);
+    summary <@ Sim(V).simulate(s);
     HybOrcl.l <- HybOrcl.l + 1;
    }
    guess <@ D.guess(s, w,  summary);
@@ -556,8 +759,8 @@ module Dstar : ZKDistinguisher = {
 
 
 local lemma lll &m deltoid : 
-   (forall &n N, 0 <= N =>
-   Pr[ZKIdeal(Sim, V, Dstar).run(s, w, N) @ &n : res]
+   (forall &n,
+   Pr[ZKIdeal(Sim, V, Dstar).run(s, w) @ &n : res]
     - Pr[ZKReal(P, V, Dstar).run(s, w) @ &n : res] 
            < deltoid) =>
    Pr[HybGame(A1,Ob1,L(Ob1)).main() @ &m : res]
@@ -589,7 +792,7 @@ have ko : exists &n, deltoid <= Pr[Amem.run1() @ &n : res] - Pr[Amem.run2() @ &n
 apply (o_o Amem &m).  auto.
 elim ko. move => &n. move => q.
 have ok : Pr[Amem.run1() @ &n : res] - Pr[Amem.run2() @ &n : res] < deltoid.
-have -> : Pr[Amem.run1() @ &n : res] = Pr[ZKIdeal(Sim, V, Dstar).run(s, w, n) @ &n : res].
+have -> : Pr[Amem.run1() @ &n : res] = Pr[ZKIdeal(Sim, V, Dstar).run(s, w) @ &n : res].
 byequiv. proc.         
 inline Dstar.guess. wp.
 seq 3 6: (={glob V} /\ summary{1} = summary0{2}). sim. wp.
@@ -604,30 +807,30 @@ seq 6 9: (={glob V} /\ summary{1} = summary0{2}). sim. wp.
 call (_:true). call (_:true).  call (_:true).  call (_:true). skip.
 progress. smt. smt. smt.  call D_guess_prop. skip. auto.
 auto.  auto. 
-apply (zk_ass  &n n _ ). smt. smt.
+apply (zk_ass  &n ). smt. 
 qed.
 
 
 
 
 lemma zk_seq &m deltoid : 
-   (forall &n N, 0 <= N =>
-   Pr[ZKIdeal(Sim, V, Dstar).run(s, w, N) @ &n : res]
+   (forall &n,
+   Pr[ZKIdeal(Sim, V, Dstar).run(s, w) @ &n : res]
     - Pr[ZKReal(P, V, Dstar).run(s, w) @ &n : res] 
            < deltoid) =>
 
-   Pr[ZKIdeal(SimAmp(Sim), V, D).run(s, w, n) @ &m : res]
+   Pr[ZKIdeal(SimAmp(Sim), V, D).run(s, w) @ &m : res]
         - Pr[ZKRealAmp(P, V, D).run(s, w) @ &m : res]
           < n%r * deltoid.
 move => zk_ass.
-have -> : Pr[ZKIdeal(SimAmp(Sim), V, D).run(s, w, n) @ &m : res]
+have -> : Pr[ZKIdeal(SimAmp(Sim), V, D).run(s, w) @ &m : res]
  = Pr[Ln(Ob,A).main() @ &m : res].
 byequiv (_:   
   (glob V){2} = (glob V){m} /\ ={glob Sim}/\
   (statement{1}, witness{1}, n{1}) = (s, w, n) /\
    (glob V){1} = (glob V){m} ==> _). proc. inline*. wp. sp.
 seq 2 1 : (={glob V, summary} /\ statement{1} = s{2} /\ witness{1} = w{2}).   simplify. wp.
-while (={i, glob V, glob Sim} /\ summary0{1} = summary{2} /\ statement0{1} = s /\   N{1} = ZeroKnowledgeTheory.n).
+while (={i, glob V, glob Sim} /\ summary0{1} = summary{2} /\ statement0{1} = s ).
 wp. call (_: ={glob V}). sim. sim. sim. sim. wp.  skip. progress.
  skip. progress.  call D_guess_prop. skip. auto. auto. auto.
 have -> : Pr[ZKRealAmp(P, V, D).run(s, w) @ &m : res]
@@ -647,227 +850,6 @@ qed.
 
 end section.
 
-end ZeroKnowledgeTheory.
+end SequentialCompositionZK.
 
-
-
-abstract theory OneShotSimulator.
-    op zk_error : statement -> int -> real.
-
-
-    require OneToManyZK.
-    clone import OneToManyZK as OMZK with type prob <- statement,
-                                          type wit <- witness,
-                                          type sbits <- adv_summary,
-                                          type event <- bool,
-
-                                          op E <- (fun x => fst x),
-                                          op fevent <- false
-
-   rename "Simulator1" as "Simulator1NP".
-
-
-    module ZKD(P : HonestProver, V : MaliciousVerifier, D : ZKDistinguisher) = {
-      proc main(Ny : statement, w : witness) = {
-        var c,b,r,result,rb;
-        c <@ P.commitment(Ny,w);
-        b <@ V.challenge(Ny,c);
-        r <@ P.response(b);
-        result <@ V.summitup(Ny,r);
-        rb <@ D.guess(Ny,w,result);
-        return rb;
-      }
-    }.
-
-
-
-     module  Simulator(S : Simulator1)(V : RewMaliciousVerifier)  = {
-       module M = MW.IFB.IM.W(S(V))
-       proc simulate(statement : statement, n : int) :
-         adv_summary = {
-            var r;
-            r <@ M.whp(fst, (statement),1,n,(false,witness));
-            return r.`2;
-       }
-     }.
-
-
-    theory ComputationalZK.
-
-    section.
-    op negl : real.
-
-    declare module HonestProver <: HonestProver.
-    declare module Sim1 <: Simulator1 {-MW.IFB.IM.W, -MW.IFB.DW}.
-    declare module V <: RewMaliciousVerifier {-Sim1, -MW.IFB.IM.W, -HonestProver, -MW.IFB.DW}.
-    declare module D <: ZKDistinguisher{ -MW.IFB.DW, -MW.IFB.IM.W} .
-
-
-    declare axiom sim1_run_ll : forall (V0 <: RewMaliciousVerifier),
-         islossless V0.challenge => islossless V0.summitup => islossless Sim1(V0).run.
-    declare axiom V_summitup_ll  : islossless V.summitup.
-    declare axiom V_challenge_ll : islossless V.challenge.
-    declare axiom D_guess_ll     : islossless D.guess.
-
-
-    declare axiom V_rew :  (exists (f : glob V -> sbits),
-         injective f /\
-         (forall &m, Pr[ V.getState() @ &m : (glob V) = ((glob V){m})
-                                          /\ res = f ((glob V){m} ) ] = 1%r) /\
-         (forall &m b (x: glob V), b = f x =>
-           Pr[V.setState(b) @ &m : glob V = x] = 1%r) /\
-         islossless V.setState).
-
-
-    declare axiom sim1_rew_ph : forall (x : (glob Sim1(V))),
-                  phoare[ Sim1(V).run : (glob Sim1(V)) = x ==> ! fst res => (glob Sim1(V)) = x] = 1%r.
-
-
-    declare axiom D_guess_prop : equiv[ D.guess ~ D.guess : ={glob V, arg} ==> ={res} ].
-
-     lemma computational_statisticalVpoly_zk stat wit N p0 negl &m:
-        zk_relation stat wit =>
-
-        `|Pr[W0(Sim1(V), D).run(stat, wit) @ &m : fst res.`2 /\ res.`1] /
-             Pr[Sim1(V).run(stat) @ &m : fst res]
-         - Pr[ ZKD(HonestProver,V,D).main(stat,wit) @ &m : res ]| <= negl =>
-
-        0 <= N =>
-
-        p0 <= Pr[Sim1(V).run(stat) @ &m : res.`1] =>
-
-        let real_prob = Pr[ZKReal(HonestProver, V, D).run(stat, wit) @ &m : res] in
-        let ideal_prob = Pr[ZKIdeal(Simulator(Sim1), V, D).run(stat, wit, N) @ &m : res] in
-          `|real_prob - ideal_prob| <= negl + 2%r * (1%r - p0)^N.
-    proof. progress.
-    have ->:
-     `|Pr[ZKReal(HonestProver, V, D).run(stat, wit) @ &m : res] -
-      Pr[ZKIdeal(Simulator(Sim1), V, D).run(stat, wit, N) @ &m : res]|
-      = `|Pr[ZKIdeal(Simulator(Sim1), V, D).run(stat, wit, N) @ &m : res]
-          - Pr[ZKReal(HonestProver, V, D).run(stat, wit) @ &m : res]|. smt.
-    have ->: Pr[ZKIdeal(Simulator(Sim1), V, D).run(stat, wit, N) @ &m : res]
-     = Pr[Iter(Sim1(V), D).run(false,stat,wit,N,fst) @ &m : res.`1].
-    byequiv (_:  E{2} = fst  /\ n{1} = ea{2} /\ fevent{2} = false  /\
-      statement{1} = Ny{2} /\ witness{1} = w{2} /\
-        ={glob Sim1, glob HonestProver,  glob V, glob MW.IFB.IM.W} ==> _)  ;auto.  proc.
-    inline Iter(Sim1(V), D).WI.run. wp.  sp. simplify.
-     call D_guess_prop.
-    simplify. inline Simulator(Sim1,V).simulate. wp. sp.
-     
-    
-
-    call (_: ={glob Sim1, glob V, glob MW.IFB.IM.W}).  sim. skip. progress.
-    progress.
-    have ->: Pr[ZKReal(HonestProver, V, D).run(stat, wit) @ &m : res]
-      = Pr[ ZKD(HonestProver,V,D).main(stat,wit) @ &m : res ].
- 
-     byequiv (_:   arg{2} = (stat, wit) /\ ={glob V, glob HonestProver}
- /\
-  (glob V){2} = (glob V){m} /\
-  (glob HonestProver){2} = (glob HonestProver){m} /\
-  arg{1} = (stat, wit) /\
- 
-  (glob V){1} = (glob V){m} /\
-  (glob HonestProver){1} = (glob HonestProver){m} ==> _).
-  proc. seq  4 4 : (={glob V} /\ (statement{1}, witness{1}, summary{1}) =
-  (Ny{2}, w{2}, result{2})). sim. call D_guess_prop. skip. auto. auto. auto.
-    apply (one_to_many_zk  (Sim1(V)) D _  _ _ _ _ &m  stat wit p0 negl N
-       Pr[ZKD(HonestProver, V, D).main(stat, wit) @ &m : res]  _ _ _).
-
-    conseq D_guess_prop. auto.
-
-    apply (sim1_run_ll V). apply V_challenge_ll. apply V_summitup_ll.
-    apply sim1_rew_ph. apply D_guess_ll.
-    auto. auto. auto. smt. auto.
-    qed.
-    end section.
-   end ComputationalZK.
-
-
-   
-   theory StatisticalZK.
-
-    op negl : real.
-
-    section.
-    declare module HonestProver <: HonestProver.
-    declare module Sim1 <: Simulator1 {-MW.IFB.IM.W, -MW.IFB.DW}.
-    declare module V <: RewMaliciousVerifier {-Sim1, -MW.IFB.IM.W, -HonestProver, -MW.IFB.DW}.
-    declare module D <: ZKDistinguisher{-MW.IFB.IM.W,  -MW.IFB.DW}.
-
-    declare axiom sim1_run_ll : forall (V0 <: RewMaliciousVerifier), islossless V0.challenge
-                                  => islossless V0.summitup => islossless Sim1(V0).run.
-    declare axiom V_summitup_ll  : islossless V.summitup.
-    declare axiom V_challenge_ll : islossless V.challenge.
-    declare axiom D_guess_ll     : islossless D.guess.
-
-    declare axiom V_rew :  (exists (f : glob V -> sbits),
-         injective f /\
-         (forall &m, Pr[ V.getState() @ &m : (glob V) = ((glob V){m})
-                                          /\ res = f ((glob V){m} ) ] = 1%r) /\
-         (forall &m b (x: glob V), b = f x =>
-           Pr[V.setState(b) @ &m : glob V = x] = 1%r) /\
-         islossless V.setState).
-
-
-    declare axiom sim1_rew_ph :
-         forall (x : (glob Sim1(V))),
-                  phoare[ Sim1(V).run : (glob Sim1(V)) = x ==> !fst res => (glob Sim1(V)) = x] = 1%r.
-
-   
-    declare axiom qqq &m (p : statement) (w : witness)
-      (D <: ZKDistinguisher)
-         (V <: RewMaliciousVerifier{-D, -HonestProver}):
-       islossless D.guess =>
-       islossless V.summitup =>
-       islossless V.challenge =>
-      (exists (f : glob V -> sbits),
-         injective f /\
-         (forall &m, Pr[ V.getState() @ &m : (glob V) = ((glob V){m})
-                                          /\ res = f ((glob V){m} ) ] = 1%r) /\
-         (forall &m b (x: glob V), b = f x =>
-           Pr[V.setState(b) @ &m : glob V = x] = 1%r) /\
-         islossless V.setState) =>
-       zk_relation p w =>
-        `|Pr[W0(Sim1(V), D).run(p, w) @ &m : fst res.`2 /\ res.`1] /
-             Pr[Sim1(V).run(p) @ &m : fst res]
-                  - Pr[ ZKD(HonestProver,V,D).main(p,w) @ &m : res ]| <= negl.
-
-
-    declare axiom D_guess_prop : equiv[ D.guess ~ D.guess : ={glob V, arg} ==> ={res} ].
-    
-     lemma statistical_zk stat wit N p0 &m:
-        zk_relation stat wit => 0 <= N =>
-        p0 <= Pr[Sim1(V).run(stat) @ &m : res.`1] =>
-        let real_prob = Pr[ZKReal(HonestProver, V, D).run(stat, wit) @ &m : res] in
-        let ideal_prob = Pr[ZKIdeal(Simulator(Sim1), V, D).run(stat, wit, N) @ &m : res] in
-          `|real_prob - ideal_prob| <= negl + 2%r * (1%r - p0)^N.
-    proof. progress.
-    have ->:
-     `|Pr[ZKReal(HonestProver, V, D).run(stat, wit) @ &m : res] -
-      Pr[ZKIdeal(Simulator(Sim1), V, D).run(stat, wit, N) @ &m : res]|
-      = `|Pr[ZKIdeal(Simulator(Sim1), V, D).run(stat, wit, N) @ &m : res]
-          - Pr[ZKReal(HonestProver, V, D).run(stat, wit) @ &m : res]|. smt.
-    have ->: Pr[ZKIdeal(Simulator(Sim1), V, D).run(stat, wit, N) @ &m : res]
-     = Pr[Iter(Sim1(V), D).run(false,stat,wit,N,fst) @ &m : res.`1].
-    byequiv (_:  E{2} = fst /\ n{1} = ea{2} /\ fevent{2} = false  /\
-      statement{1} = Ny{2} /\ witness{1} = w{2} /\
-        ={glob Sim1, glob HonestProver,  glob V, glob MW.IFB.IM.W} ==> _)  ;auto. proc.
-    inline Iter(Sim1(V), D).WI.run. wp.  sp. simplify.
-    call D_guess_prop.  simplify. inline Simulator(Sim1,V).simulate. wp. sp.
-    call (_: ={glob Sim1, glob V, glob MW.IFB.IM.W}).  sim. skip. progress.
-    have ->: Pr[ZKReal(HonestProver, V, D).run(stat, wit) @ &m : res]
-      = Pr[ ZKD(HonestProver,V,D).main(stat,wit) @ &m : res ].
-byequiv(_: arg{2} = (stat,  wit) /\   arg{1} = (stat, wit) /\  ={glob V, glob HonestProver} ==> _).
-proc. call D_guess_prop. sim. auto. auto.
-    apply (one_to_many_zk (Sim1(V)) D _ _ _ _ _ &m stat wit p0 negl N
-    Pr[ZKD(HonestProver, V, D).main(stat, wit) @
- &m : res]  _ _ _
-  ) . conseq D_guess_prop. auto.
-  apply (sim1_run_ll V).  apply V_challenge_ll. apply V_summitup_ll. apply sim1_rew_ph. apply D_guess_ll. auto.
-    apply (qqq &m stat wit  D V);auto.  apply D_guess_ll. apply V_summitup_ll. apply V_challenge_ll. apply V_rew. apply H0. smt.  auto.
-    qed.
-   end section.
-   end StatisticalZK.
-end OneShotSimulator.
 
